\documentclass{cslessonsolutions}

\lessonnum{2}
\title{A Quick Overview of Summations}

\begin{document}
\maketitle
\subsection*{\textit{Warmup}}
\begin{enumerate}[listparindent=0.7cm, align=left]
\item Explain what the expression $\sum^n_{i=0}a_i$ means.\\
The expression means the sum of the terms $a_i$ where $i$ is from 0 to $n$.
\item Express the sum \begin{equation*}\sum^4_{k=1}a_k\end{equation*} in expanded sum notation.
\item Expand the triple sum \begin{equation*}\sum_{1 \leq i < j < k \leq n}a_{ijk}\end{equation*} as an expression with three summations.
\item Evaluate the following summations
\begin{enumerate}[label=(\alph*), listparindent=0.7cm, align=left]
    \item $\sum^3_{j=0}2^j$
    \item $\sum^5_{k=1}(2k-3)$
    \item $\sum^{100}_{j=1}j$
    \item $\sum^{4}_{j=0}{\frac{24}{j!}}$
    \item $\sum^{90}_{i=1}{(-2i^2+3j-5)}$
\end{enumerate}
\end{enumerate}

\subsection*{\textit{Homework}}
\begin{enumerate}[listparindent=0.7cm, align=left]
\item Solve the following recurrence using summation
\begin{align*}
    T_0&=5;\\
    2T_n&=nT_{n-1}+3n!
\end{align*}
\item Find the closed-form expression for the following sums
\begin{enumerate}[label=(\alph*), listparindent=0.7cm, align=left]
\item $\sum^n_{i=1}(2k-1)$
\item $\sum^n_{k=1}{i^{2x+1}}$
\end{enumerate}
\end{enumerate}

\subsection*{\textit{Challenge}}
\begin{enumerate}[label=(\alph*), listparindent=0.7cm, align=left]
\item Evaluate the sum $\sum^n_{k=1}(-1)^2k/(4k^2-1)$
\end{enumerate}

\end{document}